src3.0/Transforms/laa.v
@@ -15,6 +15,7 @@ Require Import mem2reg.
 Require Import program_sim.
 Require Import memory_props.
 Require Import trans_tactic.
+Require Import top_sim.
 
 Definition laa (lid: id) (cs2:cmds) (b:block) (pinfo:PhiInfo) : Prop :=
 blockInFdefB b (PI_f pinfo) = true /\
@@ -434,24 +435,39 @@ Definition block_simulation (pinfo: PhiInfo) (laainfo: LAAInfo pinfo) f1 b1 b2
     subst_block (LAA_lid pinfo laainfo) [! pinfo !] b1 = b2
   else b1 = b2.
 
-Definition products_simulation (pinfo: PhiInfo) (laainfo: LAAInfo pinfo) Ps1 Ps2
-  : Prop :=
-List.Forall2
-  (fun P1 P2 =>
-   match P1, P2 with
-   | product_fdef f1, product_fdef f2 => fdef_simulation pinfo laainfo f1 f2
-   | _, _ => P1 = P2
-   end) Ps1 Ps2.
+Lemma fdef_simulation__eq_fheader: forall pinfo laainfo f1 f2
+  (H: fdef_simulation pinfo laainfo f1 f2),
+  fheaderOfFdef f1 = fheaderOfFdef f2.
+Proof.
+  unfold fdef_simulation.
+  intros.
+  destruct (fdef_dec (PI_f pinfo) f1); inv H; auto.
+    destruct (PI_f pinfo) as [fh b]; simpl; auto.
+Qed.
 
-Definition system_simulation (pinfo: PhiInfo) (laainfo: LAAInfo pinfo) S1 S2
-  : Prop :=
-List.Forall2
-  (fun M1 M2 =>
-   match M1, M2 with
-   | module_intro los1 nts1 Ps1, module_intro los2 nts2 Ps2 =>
-       los1 = los2 /\ nts1 = nts2 /\
-       products_simulation pinfo laainfo Ps1 Ps2
-   end) S1 S2.
+Lemma fdef_simulation__det_right: forall pinfo laainfo f f1 f2,
+  fdef_simulation pinfo laainfo f f1 ->
+  fdef_simulation pinfo laainfo f f2 ->
+  f1 = f2.
+Proof.
+  unfold fdef_simulation.
+  intros.
+  destruct_if; congruence.
+Qed.
+
+Definition Fsim (pinfo: PhiInfo) (laainfo: LAAInfo pinfo) := mkFunSim 
+(fdef_simulation pinfo laainfo)
+(fdef_simulation__eq_fheader pinfo laainfo)
+(fdef_simulation__det_right pinfo laainfo)
+.
+
+Definition products_simulation (pinfo: PhiInfo) (laainfo: LAAInfo pinfo) 
+  Ps1 Ps2 : Prop :=
+@TopSim.products_simulation (Fsim pinfo laainfo) Ps1 Ps2.
+
+Definition system_simulation (pinfo: PhiInfo) (laainfo: LAAInfo pinfo) 
+  S1 S2 : Prop :=
+@TopSim.system_simulation (Fsim pinfo laainfo) S1 S2.
 
 Definition phis_simulation (pinfo: PhiInfo) (laainfo: LAAInfo pinfo) (f1:fdef)
   ps1 ps2 : Prop :=
@@ -868,29 +884,6 @@ Definition pars_simulation (pinfo: PhiInfo) (laainfo: LAAInfo pinfo) (f1:fdef)
   else ps1 = ps2.
 
 (* same to las' *)
-Lemma products_simulation__fdef_simulation : forall pinfo laainfo Ps1 Ps2 fid f1
-  f2,
-  lookupFdefViaIDFromProducts Ps2 fid = Some f2 ->
-  lookupFdefViaIDFromProducts Ps1 fid = Some f1 ->
-  products_simulation pinfo laainfo Ps1 Ps2 ->
-  fdef_simulation pinfo laainfo f1 f2.
-Admitted. (* prod sim *)
-
-(* same to las' *)
-Lemma lookupFdefViaPtr__simulation : forall pinfo laainfo Ps1 Ps2 fptr f1 f2 fs,
-  OpsemAux.lookupFdefViaPtr Ps2 fs fptr = Some f2 ->
-  products_simulation pinfo laainfo Ps1 Ps2 ->
-  OpsemAux.lookupFdefViaPtr Ps1 fs fptr = Some f1 ->
-  fdef_simulation pinfo laainfo f1 f2.
-Proof.
-  intros.
-  unfold OpsemAux.lookupFdefViaPtr in *.
-  remember (OpsemAux.lookupFdefViaGVFromFunTable fs fptr) as R2.
-  destruct R2 as [fid|]; inv H1. simpl in H.
-  eapply products_simulation__fdef_simulation in H0; eauto.
-Qed.
-
-(* same to las' *)
 Lemma fdef_simulation__entry_block_simulation: forall pinfo laainfo F1 F2 B1 B2,
   fdef_simulation pinfo laainfo F1 F2 ->
   getEntryBlock F1 = ret B1 ->
@@ -1046,22 +1039,6 @@ Proof.
   eapply params2GVs_sim_aux; eauto.
     exists nil. auto.
 Qed.
-
-(* same to las' *)
-Lemma lookupFdefViaPtr__simulation_l2r : forall pinfo laainfo Ps1 Ps2 fptr f1 fs,
-  products_simulation pinfo laainfo Ps1 Ps2 ->
-  OpsemAux.lookupFdefViaPtr Ps1 fs fptr = Some f1 ->
-  exists f2,
-    OpsemAux.lookupFdefViaPtr Ps2 fs fptr = Some f2 /\
-    fdef_simulation pinfo laainfo f1 f2.
-Admitted. (* fsim *)
-
-(* same to las' *)
-Lemma lookupExFdecViaPtr__simulation_l2r : forall pinfo laainfo Ps1 Ps2 fptr f fs,
-  products_simulation pinfo laainfo Ps1 Ps2 ->
-  OpsemAux.lookupExFdecViaPtr Ps1 fs fptr = Some f ->
-  OpsemAux.lookupExFdecViaPtr Ps2 fs fptr = Some f.
-Admitted. (* fsim *)
 
 (* same to las' *)
 Ltac destruct_ctx_return :=
@@ -1593,8 +1570,8 @@ Case "sCall".
   subst. clear H.
 
   assert (Hfsim1:=Hpsim).
-  eapply lookupFdefViaPtr__simulation in Hfsim1; eauto.
-
+  eapply TopSim.lookupFdefViaPtr__simulation in Hfsim1; eauto.
+  simpl in Hfsim1.
   assert (Hbsim1:=Hfsim1).
   eapply fdef_simulation__entry_block_simulation in Hbsim1; eauto.
   assert (Hbsim1':=Hbsim1).
@@ -1624,7 +1601,7 @@ Case "sCall".
   subst. clear H.
   clear - H29 H1 Hpsim.
 
-  eapply lookupFdefViaPtr__simulation_l2r in H1; eauto.
+  eapply TopSim.lookupFdefViaPtr__simulation_l2r in H1; eauto.
   destruct H1 as [f2 [H1 H2]].
   apply OpsemAux.lookupExFdecViaPtr_inversion in H29.
   apply OpsemAux.lookupFdefViaPtr_inversion in H1.
@@ -1668,7 +1645,8 @@ Case "sExCall".
     H1: OpsemAux.lookupExFdecViaPtr ?Ps _ _ = _,
     H30: OpsemAux.lookupFdefViaPtr ?Ps2 _ _ = _ |- _ =>
     clear - H30 H1 Hpsim;
-    eapply lookupExFdecViaPtr__simulation_l2r in H1; eauto;
+    eapply TopSim.lookupExFdecViaPtr__simulation_l2r in H1; eauto;
+    simpl in Hpsim;
     apply OpsemAux.lookupExFdecViaPtr_inversion in H1;
     apply OpsemAux.lookupFdefViaPtr_inversion in H30;
     destruct H1 as [fn [J1 [J2 J3]]];
@@ -1688,7 +1666,7 @@ Case "sExCall".
   subst. clear H.
 
   assert (Hlkdec:=Hpsim).
-  eapply lookupExFdecViaPtr__simulation_l2r in Hlkdec; eauto.
+  eapply TopSim.lookupExFdecViaPtr__simulation_l2r in Hlkdec; eauto.
 
   assert (gvss = gvss0) as EQ.
     inv_mfalse; symmetry_ctx.
@@ -1721,21 +1699,20 @@ Lemma s_genInitState__laa_State_simulation: forall pinfo laainfo S1 S2 main
     State_simulation pinfo laainfo cfg1 IS1 cfg2 IS2.
 Admitted. (* laainfo *)
 
-Lemma s_isFinialState__laa_State_simulation: forall pinfo laainfo cfg1 FS1 cfg2
-  FS2 r (Hstsim : State_simulation pinfo laainfo cfg1 FS1 cfg2 FS2)
-  (Hfinal: Opsem.s_isFinialState cfg2 FS2 = ret r),
-  Opsem.s_isFinialState cfg1 FS1 = ret r.
-Admitted. (* sim *)
-
-Lemma opsem_s_isFinialState__laa_State_simulation: forall
+Lemma s_isFinialState__laa_State_simulation: forall
   pinfo laainfo cfg1 FS1 cfg2 FS2
   (Hstsim : State_simulation pinfo laainfo cfg1 FS1 cfg2 FS2),
   Opsem.s_isFinialState cfg1 FS1 = Opsem.s_isFinialState cfg2 FS2.
 Admitted. (* sim *)
 
-Lemma undefined_state__laa_State_simulation: forall pinfo laainfo cfg1 St1 cfg2
+Lemma undefined_state__laa_State_simulation_l2r: forall pinfo laainfo cfg1 St1 cfg2
   St2 (Hstsim : State_simulation pinfo laainfo cfg1 St1 cfg2 St2),
   OpsemPP.undefined_state cfg1 St1 -> OpsemPP.undefined_state cfg2 St2.
+Admitted. (* sim *)
+
+Lemma undefined_state__laa_State_simulation_r2l: forall pinfo laainfo cfg1 St1 cfg2
+  St2 (Hstsim : State_simulation pinfo laainfo cfg1 St1 cfg2 St2),
+  OpsemPP.undefined_state cfg2 St2 -> OpsemPP.undefined_state cfg1 St1.
 Admitted. (* sim *)
 
 Lemma sop_star__laa_State_simulation: forall pinfo laainfo cfg1 IS1 cfg2 IS2 tr
@@ -1764,7 +1741,7 @@ Proof.
     assert (J:=Hwfpp).
     apply OpsemPP.progress in J; auto.
     destruct J as [Hfinal1 | [[IS1' [tr0 Hop1]] | Hundef1]].
-      apply opsem_s_isFinialState__laa_State_simulation in Hstsim.
+      apply s_isFinialState__laa_State_simulation in Hstsim.
       rewrite Hstsim in Hfinal1.
       contradict H; eauto using s_isFinialState__stuck.
 
@@ -1787,7 +1764,7 @@ Proof.
       exists FS1.
       split; eauto.
 
-      eapply undefined_state__laa_State_simulation in Hstsim; eauto.
+      eapply undefined_state__laa_State_simulation_l2r in Hstsim; eauto.
       contradict H; eauto using undefined_state__stuck.
 Qed.
 
@@ -1825,120 +1802,6 @@ Proof.
     apply LAA_value__dominates__LAA_lid.
 Qed.
 
-Lemma laa_sim: forall (los : layouts) (nts : namedts) (fh : fheader)
-  (dones : list id) (pinfo : PhiInfo) (main : id) (VarArgs : list (GVsT DGVs))
-  (bs1 : list block) (l0 : l) (ps0 : phinodes) (cs0 : cmds) (tmn0 : terminator)
-  (bs2 : list block) (Ps1 : list product) (Ps2 : list product) (v : value)
-  (cs : cmds)
-  (Hst : ret inr (v, cs) = find_init_stld cs0 (PI_id pinfo) dones)
-  (i1 : id) (Hld : ret inl i1 = find_next_stld cs (PI_id pinfo))
-  (Heq: PI_f pinfo = fdef_intro fh (bs1 ++ block_intro l0 ps0 cs0 tmn0 :: bs2))
-  (Hwfpi: WF_PhiInfo pinfo)
-  (HwfS :
-     wf_system 
-       [module_intro los nts
-         (Ps1 ++
-          product_fdef
-            (fdef_intro fh (bs1 ++ block_intro l0 ps0 cs0 tmn0 :: bs2))
-          :: Ps2)]),
-  program_sim
-     [module_intro los nts
-        (Ps1 ++
-         product_fdef
-           (subst_fdef i1 v
-              (fdef_intro fh (bs1 ++ block_intro l0 ps0 cs0 tmn0 :: bs2)))
-         :: Ps2)]
-     [module_intro los nts
-        (Ps1 ++
-         product_fdef
-           (fdef_intro fh (bs1 ++ block_intro l0 ps0 cs0 tmn0 :: bs2)) :: Ps2)]
-     main VarArgs.
-Proof.
-  intros.
-  assert (blockInFdefB (block_intro l0 ps0 cs0 tmn0) (PI_f pinfo) = true)
-    as HBinF.
-    rewrite Heq. simpl. apply InBlocksB_middle.
-  eapply find_st_ld__laainfo in HBinF; eauto.
-  destruct HBinF as [EQ [laainfo [J1 J2]]]; subst.
-  assert (Huniq:=HwfS). apply wf_system__uniqSystem in Huniq; auto.
-  assert (system_simulation pinfo laainfo
-     [module_intro los nts
-        (Ps1 ++
-         product_fdef
-           (fdef_intro fh (bs1 ++ block_intro l0 ps0 cs0 tmn0 :: bs2)) :: Ps2)]
-     [module_intro los nts
-        (Ps1 ++
-         product_fdef
-           (subst_fdef (LAA_lid pinfo laainfo) [! pinfo !]
-              (fdef_intro fh (bs1 ++ block_intro l0 ps0 cs0 tmn0 :: bs2)))
-         :: Ps2)]) as Hssim.
-    unfold system_simulation.
-    constructor; auto.
-    repeat split; auto.
-    unfold products_simulation.
-    simpl in Huniq. destruct Huniq as [[_ [_ Huniq]] _].
-    apply uniq_products_simulation; auto.
-  assert (uniqFdef (PI_f pinfo)) as HuniqF.
-    admit. (* wfF *)
-  constructor.
-    intros tr t Hconv.
-    inv Hconv.
-    eapply s_genInitState__laa_State_simulation in H; eauto.
-    destruct H as [cfg1 [IS1 [Hinit Hstsim]]].    
-    assert (OpsemPP.wf_Config cfg1 /\ OpsemPP.wf_State cfg1 IS1) as Hwfst. 
-      eapply s_genInitState__opsem_wf; eauto.
-    assert (id_rhs_val.wf_State (value_id (LAA_lid pinfo laainfo))
-              [! pinfo !] (PI_f pinfo) cfg1 IS1) as Hisrhsval.
-      eapply s_genInitState__id_rhs_val; eauto using LAA_substable_values.
-    assert (exists maxb,
-              MemProps.wf_globals maxb (OpsemAux.Globals cfg1) /\ 0 <= maxb /\
-              Promotability.wf_State maxb pinfo cfg1 IS1) as Hprom.
-      eapply Promotability.s_genInitState__wf_globals_promotable; eauto.
-    destruct Hprom as [maxb [Hwfg [Hless Hprom]]].
-    remember (laainfo__alinfo pinfo laainfo) as R.
-    destruct R as [alinfo Hp].
-    assert (substable_values (OpsemAux.CurTargetData cfg1) (OpsemAux.Globals cfg1)
-      (PI_f pinfo) (value_id (LAA_lid pinfo laainfo)) [! pinfo !]) as Hdom.
-      assert ((los,nts) = OpsemAux.CurTargetData cfg1) as EQ.
-        admit. (* prop of initState *)
-      rewrite <- EQ.
-      eapply LAA_substable_values; eauto.
-    assert (alive_alloca.wf_State pinfo alinfo cfg1 IS1) as Halst.
-      eapply s_genInitState__alive_alloca; eauto.
-    eapply sop_star__laa_State_simulation in Hstsim; eauto; try tauto.
-    destruct Hstsim as [FS1 [Hopstar1 Hstsim']].
-    eapply s_isFinialState__laa_State_simulation in Hstsim'; eauto.
-    econstructor; eauto.
-
-    intros tr Hdiv.
-    inv Hdiv.
-    eapply s_genInitState__laa_State_simulation in H; eauto.
-    destruct H as [cfg1 [IS1 [Hinit Hstsim]]].  
-    assert (OpsemPP.wf_Config cfg1 /\ OpsemPP.wf_State cfg1 IS1) as Hwfst. 
-      eapply s_genInitState__opsem_wf; eauto.
-    assert (id_rhs_val.wf_State (value_id (LAA_lid pinfo laainfo))
-              [! pinfo !] (PI_f pinfo) cfg1 IS1) as Hisrhsval.
-      eapply s_genInitState__id_rhs_val; eauto using LAA_substable_values.
-    assert (exists maxb,
-              MemProps.wf_globals maxb (OpsemAux.Globals cfg1) /\ 0 <= maxb /\
-              Promotability.wf_State maxb pinfo cfg1 IS1) as Hprom.
-      eapply Promotability.s_genInitState__wf_globals_promotable; eauto.
-    destruct Hprom as [maxb [Hwfg [Hless Hprom]]].
-    remember (laainfo__alinfo pinfo laainfo) as R.
-    destruct R as [alinfo Hp].
-    assert (substable_values (OpsemAux.CurTargetData cfg1) (OpsemAux.Globals cfg1)
-      (PI_f pinfo) (value_id (LAA_lid pinfo laainfo)) [! pinfo !]) as Hdom.
-      assert ((los,nts) = OpsemAux.CurTargetData cfg1) as EQ.
-        admit. (* prop of initState *)
-      rewrite <- EQ.
-      eapply LAA_substable_values; eauto.
-    assert (alive_alloca.wf_State pinfo alinfo cfg1 IS1) as Halst.
-      eapply s_genInitState__alive_alloca; eauto.
-    eapply sop_div__laa_State_simulation in Hstsim; eauto; try tauto.
-    destruct Hstsim as [FS1 Hopdiv1].
-    econstructor; eauto.
-Qed.
-
 Lemma laa_wfS: forall (los : layouts) (nts : namedts) (fh : fheader)
   (dones : list id) (pinfo: PhiInfo)
   (bs1 : list block) (l0 : l) (ps0 : phinodes) (cs0 : cmds) (tmn0 : terminator)
@@ -1962,6 +1825,131 @@ Lemma laa_wfS: forall (los : layouts) (nts : namedts) (fh : fheader)
            (fdef_intro fh (bs1 ++ block_intro l0 ps0 cs0 tmn0 :: bs2))) :: Ps2)].
 Proof.
 Admitted. (* WF prev *)
+
+Lemma laa_sim: forall (los : layouts) (nts : namedts) (fh : fheader)
+  (dones : list id) (pinfo : PhiInfo) (main : id) (VarArgs : list (GVsT DGVs))
+  (bs1 : list block) (l0 : l) (ps0 : phinodes) (cs0 : cmds) (tmn0 : terminator)
+  (bs2 : list block) (Ps1 : list product) (Ps2 : list product) (v : value)
+  (cs : cmds)
+  (Hst : ret inr (v, cs) = find_init_stld cs0 (PI_id pinfo) dones)
+  (i1 : id) (Hld : ret inl i1 = find_next_stld cs (PI_id pinfo))
+  (Heq: PI_f pinfo = fdef_intro fh (bs1 ++ block_intro l0 ps0 cs0 tmn0 :: bs2))
+  (Hwfpi: WF_PhiInfo pinfo)
+  S2 (Heq2: S2=[module_intro los nts
+                (Ps1 ++
+                  product_fdef
+                    (fdef_intro fh (bs1 ++ block_intro l0 ps0 cs0 tmn0 :: bs2))
+                 :: Ps2)])
+  (Hok: defined_program S2 main VarArgs)
+  (HwfS : wf_system S2),
+  program_sim
+     [module_intro los nts
+        (Ps1 ++
+         product_fdef
+           (subst_fdef i1 v
+              (fdef_intro fh (bs1 ++ block_intro l0 ps0 cs0 tmn0 :: bs2)))
+         :: Ps2)]
+     S2 main VarArgs.
+Proof.
+  intros.
+  assert (blockInFdefB (block_intro l0 ps0 cs0 tmn0) (PI_f pinfo) = true)
+    as HBinF.
+    rewrite Heq. simpl. apply InBlocksB_middle.
+  eapply find_st_ld__laainfo in HBinF; eauto.
+  destruct HBinF as [EQ [laainfo [J1 J2]]]; subst.
+  assert (Huniq:=HwfS). apply wf_system__uniqSystem in Huniq; auto.
+  assert (system_simulation pinfo laainfo
+     [module_intro los nts
+        (Ps1 ++
+         product_fdef
+           (fdef_intro fh (bs1 ++ block_intro l0 ps0 cs0 tmn0 :: bs2)) :: Ps2)]
+     [module_intro los nts
+        (Ps1 ++
+         product_fdef
+           (subst_fdef (LAA_lid pinfo laainfo) [! pinfo !]
+              (fdef_intro fh (bs1 ++ block_intro l0 ps0 cs0 tmn0 :: bs2)))
+         :: Ps2)]) as Hssim.
+    constructor; auto.
+    repeat split; auto.
+    simpl in Huniq. destruct Huniq as [[_ [_ Huniq]] _].
+    unfold TopSim.products_simulation. unfold fsim. unfold Fsim.
+    apply uniq_products_simulation; auto.
+  assert (uniqFdef (PI_f pinfo)) as HuniqF.
+    admit. (* wfF *)
+  constructor; auto.
+    intros tr t Hconv.
+    inv Hconv.
+
+Ltac laa_sim_init :=
+match goal with
+| H: Opsem.s_genInitState [module_intro ?los ?nts _] _ _ _ = _,  
+  pinfo: PhiInfo, laainfo: LAAInfo _
+  |- _ =>
+    eapply s_genInitState__laa_State_simulation in H; eauto;
+    destruct H as [cfg1 [IS1 [Hinit Hstsim]]];
+    assert (OpsemPP.wf_Config cfg1 /\ OpsemPP.wf_State cfg1 IS1) as Hwfst;
+      try solve [eapply s_genInitState__opsem_wf; eauto];
+    assert (id_rhs_val.wf_State (value_id (LAA_lid pinfo laainfo))
+              [! pinfo !] (PI_f pinfo) cfg1 IS1) as Hisrhsval;
+      try solve [eapply s_genInitState__id_rhs_val; 
+                 eauto using LAA_substable_values];
+    assert (exists maxb,
+              MemProps.wf_globals maxb (OpsemAux.Globals cfg1) /\ 0 <= maxb /\
+              Promotability.wf_State maxb pinfo cfg1 IS1) as Hprom;
+      try solve [eapply Promotability.s_genInitState__wf_globals_promotable; eauto];
+    destruct Hprom as [maxb [Hwfg [Hless Hprom]]];
+    remember (laainfo__alinfo pinfo laainfo) as R;
+    destruct R as [alinfo Hp];
+    assert (substable_values (OpsemAux.CurTargetData cfg1) (OpsemAux.Globals cfg1)
+      (PI_f pinfo) (value_id (LAA_lid pinfo laainfo)) [! pinfo !]) as Hdom;
+      try solve [
+      assert ((los,nts) = OpsemAux.CurTargetData cfg1) as EQ;
+        try solve [eapply s_genInitState__targedata; eauto];
+      rewrite <- EQ;
+      eapply LAA_substable_values; eauto
+     ];
+    assert (alive_alloca.wf_State pinfo alinfo cfg1 IS1) as Halst;
+      try solve [eapply s_genInitState__alive_alloca; eauto]
+end.
+
+    laa_sim_init.
+    eapply sop_star__laa_State_simulation in Hstsim; eauto; try tauto.
+    destruct Hstsim as [FS1 [Hopstar1 Hstsim']].
+    match goal with
+    | H1: Opsem.s_isFinialState _ _ = _ |- _ =>
+      erewrite <- s_isFinialState__laa_State_simulation in H1; eauto
+    end.
+    econstructor; eauto.
+
+    intros tr Hdiv.
+    inv Hdiv.
+    laa_sim_init.
+    eapply sop_div__laa_State_simulation in Hstsim; eauto; try tauto.
+    destruct Hstsim as [FS1 Hopdiv1].
+    econstructor; eauto.
+
+    intros tr t Hgowrong.
+    inv Hgowrong.
+    assert (OpsemPP.wf_Config cfg /\ OpsemPP.wf_State cfg t) as HwfSt.
+      eapply s_genInitState__opsem_wf in H; eauto using laa_wfS.
+      destruct H as [Hcfg2 HwfSt2].
+      apply OpsemPP.preservation_star in H0; auto.
+    assert (OpsemPP.undefined_state cfg t) as Hundef.
+      apply stuck__undefined_state in H2; try solve [auto | tauto].
+    laa_sim_init.
+    eapply sop_star__laa_State_simulation in Hstsim; eauto; try tauto.
+    destruct Hstsim as [FS1 [Hopstar1 Hstsim']].
+    eapply Promotability.preservation_star in Hprom; eauto; try tauto.
+    assert (OpsemPP.undefined_state cfg1 FS1) as Hundef'.
+      eapply undefined_state__laa_State_simulation_r2l in Hundef; 
+        try solve [eauto | tauto].
+    assert (Opsem.s_isFinialState cfg1 FS1 = merror) as Hfinal'.
+      erewrite <- s_isFinialState__laa_State_simulation in H2; 
+        try solve [eauto | tauto].
+    apply undefined_state__stuck' in Hundef'.
+    exists tr. exists FS1.
+    econstructor; eauto.
+Qed.
 
 Lemma laa_wfPI: forall (los : layouts) (nts : namedts) (fh : fheader)
   (dones : list id) (pinfo: PhiInfo)
