src3.0/Transforms/top_sim.v
@@ -1,0 +1,629 @@
+Require Import vellvm.
+Require Import genericvalues_inject.
+Require Import palloca_props.
+
+Structure FunSim := mkFunSim {
+fsim: fdef -> fdef -> Prop;
+eq_fheader: forall f1 f2
+  (H: fsim f1 f2), fheaderOfFdef f1 = fheaderOfFdef f2;
+det_right: forall f f1 f2,
+  fsim f f1 -> fsim f f2 -> f1 = f2
+}.
+
+Module TopSim.
+
+Section TopSim.
+
+Context `{FSim : FunSim}.
+
+Definition products_simulation Ps1 Ps2: Prop :=
+List.Forall2
+  (fun P1 P2 =>
+   match P1, P2 with
+   | product_fdef f1, product_fdef f2 => FSim.(fsim) f1 f2
+   | _, _ => P1 = P2
+   end) Ps1 Ps2.
+
+Definition system_simulation S1 S2: Prop :=
+List.Forall2
+  (fun M1 M2 =>
+   match M1, M2 with
+   | module_intro los1 nts1 Ps1, module_intro los2 nts2 Ps2 =>
+       los1 = los2 /\ nts1 = nts2 /\
+       products_simulation Ps1 Ps2
+   end) S1 S2.
+
+Definition module_simulation (M1 M2: module) : Prop :=
+match M1, M2 with
+| module_intro los1 nts1 Ps1, module_intro los2 nts2 Ps2 =>
+    los1 = los2 /\ nts1 = nts2 /\ 
+    products_simulation Ps1 Ps2
+end.
+
+Lemma fdef_simulation__inv: forall f1 f2,
+  FSim.(fsim) f1 f2 -> getFdefID f1 = getFdefID f2.
+Proof.
+  intros.
+  apply FSim.(eq_fheader) in H.
+  destruct f1 as [[]]; destruct f2 as [[]]; inv H; auto.
+Qed.
+
+Lemma products_simulation__fdef_simulation_l2r : forall fid Ps1 Ps2
+  (Hsim: products_simulation Ps1 Ps2) f1,
+  lookupFdefViaIDFromProducts Ps1 fid = Some f1 ->
+  exists f2,
+    lookupFdefViaIDFromProducts Ps2 fid = Some f2 /\
+    FSim.(fsim) f1 f2.
+Proof.
+  intros fid Ps1 Ps2 Hsim.
+  induction Hsim; simpl; intros.
+    inv H.
+
+    destruct x as [?|?|f];
+    destruct y as [?|?|f0]; inv H0; eauto; try congruence.
+    destruct (getFdefID f == fid); subst.
+      inv H2. simpl.
+      destruct (getFdefID f0 == getFdefID f1); eauto.
+        apply IHHsim. simpl.
+        destruct f0 as [[]], f1 as [[]].
+        apply fdef_simulation__inv in H.
+        contradict n; auto.
+    simpl.
+    destruct (getFdefID f0 == fid); subst; auto.
+      destruct f0 as [[]], f as [[]].
+      apply fdef_simulation__inv in H.
+      contradict n; auto.
+Qed.
+
+Lemma products_simulation__fdef_simulation_r2l : forall fid f2 Ps1 Ps2,
+  products_simulation Ps1 Ps2 ->
+  lookupFdefViaIDFromProducts Ps2 fid = ret f2 ->
+  exists f1,
+    lookupFdefViaIDFromProducts Ps1 fid = ret f1 /\
+    FSim.(fsim) f1 f2.
+Proof.
+  induction Ps1; simpl; intros Ps2 J1 J2.
+    inv J1. inv J2.
+
+    inv J1. simpl in J2.
+    remember (lookupFdefViaIDFromProduct y fid) as R.
+    destruct R; inv J2.
+      destruct a as [?|f0|f0]; subst; tinv HeqR.
+      destruct y as [?|?|f5]; subst; tinv HeqR.
+      simpl in HeqR. simpl.
+      destruct (getFdefID f5 == fid); inv HeqR.
+      exists f0.
+      split; auto.
+        apply fdef_simulation__inv in H1.
+        destruct (getFdefID f0 == getFdefID f5); auto.
+        rewrite H1 in n. congruence.
+
+      destruct a as [?|f0|f0]; subst; simpl; try eapply IHPs1; eauto.  
+      destruct y as [?|?|f5]; subst; tinv H1.
+      simpl in *.
+      destruct (getFdefID f5 == fid); inv HeqR.
+      eapply IHPs1 in H0; eauto.
+      destruct H0 as [f1 [J1 J2]].
+      exists f1.
+      split; auto.
+        apply fdef_simulation__inv in H1.
+        rewrite H1.
+        destruct (getFdefID f5 == fid); auto.
+          subst. congruence.
+Qed.
+
+Lemma products_simulation__fdef_simulation : forall fid Ps1 Ps2
+  (Hsim: products_simulation Ps1 Ps2) f1 f2,
+  lookupFdefViaIDFromProducts Ps2 fid = Some f2 ->
+  lookupFdefViaIDFromProducts Ps1 fid = Some f1 ->
+  FSim.(fsim) f1 f2.
+Proof.
+  intros.
+  eapply products_simulation__fdef_simulation_r2l in H; eauto.
+  destruct H as [f1' [H1 H2]].
+  uniq_result. auto.
+Qed.
+
+Lemma products_simulation__fdef_None_r2l : forall fid Ps1 Ps2,
+  products_simulation Ps1 Ps2 ->
+  lookupFdefViaIDFromProducts Ps2 fid = merror ->
+  lookupFdefViaIDFromProducts Ps1 fid = merror.
+Proof.
+  intros.
+  remember (lookupFdefViaIDFromProducts Ps1 fid) as R.
+  destruct R; auto. symmetry_ctx.
+  eapply products_simulation__fdef_simulation_l2r in HeqR; eauto.
+  destruct HeqR as [f2 [J1 J2]].
+  congruence.
+Qed.
+
+Lemma products_simulation__fdef_None_l2r : forall fid Ps1 Ps2,
+  products_simulation Ps1 Ps2 ->
+  lookupFdefViaIDFromProducts Ps1 fid = merror ->
+  lookupFdefViaIDFromProducts Ps2 fid = merror.
+Proof.
+  intros.
+  remember (lookupFdefViaIDFromProducts Ps2 fid) as R.
+  destruct R; auto. symmetry_ctx.
+  eapply products_simulation__fdef_simulation_r2l in HeqR; eauto.
+  destruct HeqR as [f2 [J1 J2]].
+  congruence.
+Qed.
+
+Lemma products_simulation__fdec_eq : forall fid Ps1 Ps2,
+  products_simulation Ps1 Ps2 ->
+  lookupFdecViaIDFromProducts Ps1 fid =
+    lookupFdecViaIDFromProducts Ps2 fid.
+Proof.
+  induction 1; simpl; auto.
+    rewrite IHForall2.
+    destruct x; subst; auto.
+    destruct y; subst; auto.
+    congruence.
+Qed.
+
+Lemma products_simulation__fdec_r2l : forall fid f Ps1 Ps2,
+  products_simulation Ps1 Ps2 ->
+  lookupFdecViaIDFromProducts Ps2 fid = ret f ->
+  lookupFdecViaIDFromProducts Ps1 fid = ret f.
+Proof.
+  intros.
+  erewrite products_simulation__fdec_eq; eauto. 
+Qed.
+
+Lemma products_simulation__fdec_l2r : forall fid f Ps1 Ps2,
+  products_simulation Ps1 Ps2 ->
+  lookupFdecViaIDFromProducts Ps1 fid = ret f ->
+  lookupFdecViaIDFromProducts Ps2 fid = ret f.
+Proof.
+  intros.
+  erewrite <- products_simulation__fdec_eq; eauto. 
+Qed.
+
+Lemma system_simulation__fdef_simulation_r2l : forall fid f2 S1 S2
+  (Hssim: system_simulation S1 S2)
+  (Hlkup: lookupFdefViaIDFromSystem S2 fid = ret f2),
+  exists f1, 
+    lookupFdefViaIDFromSystem S1 fid = ret f1 /\
+    FSim.(fsim) f1 f2.
+Proof.
+  induction 1; simpl; intros.
+    inv Hlkup.
+
+    match goal with
+    | H: match ?x with
+         | module_intro _ _ _ => 
+             match ?y with | module_intro _ _ _ => _ end
+         end |- _ => 
+        destruct x as [los1 nts1 Ps1]; destruct y as [los2 nts2 Ps2];
+        destruct H as [J1 [J2 J3]]; subst
+    end.
+    simpl in *.
+
+   destruct_match.
+     eapply products_simulation__fdef_simulation_r2l in HeqR; eauto.
+     destruct HeqR as [f1 [J1 J2]].
+     fill_ctxhole. eauto.
+
+     symmetry in HeqR.
+     eapply products_simulation__fdef_None_r2l in HeqR; eauto.
+     fill_ctxhole. eauto.
+Qed.
+
+Lemma products_simulation__eq_getFdefsIDs: forall Ps1 Ps2
+  (Hpsim: products_simulation Ps1 Ps2),
+  getFdefsIDs Ps1 = getFdefsIDs Ps2.
+Proof.
+  intros.
+  induction Hpsim; intros; auto.
+    destruct x; subst; simpl; auto.
+    destruct y; tinv H.
+    destruct f as [[]]. destruct f0 as [[]]. 
+    apply fdef_simulation__inv in H. congruence.
+Qed.
+
+Lemma products_fdef_simulation__InProductsB_forward: forall f1 f2 Ps1 Ps2,
+  products_simulation Ps1 Ps2 ->
+  InProductsB (product_fdef f1) Ps1 = true ->
+  FSim.(fsim) f1 f2 ->
+  InProductsB (product_fdef f2) Ps2 = true.
+Proof.
+  induction 1; simpl; intros; auto.
+    destruct x; subst; simpl.
+      rewrite productNEqB_intro in H1; try congruence.
+      rewrite productNEqB_intro; try congruence.
+      rewrite orb_false_l in H1.
+      rewrite orb_false_l. auto.
+
+      rewrite productNEqB_intro in H1; try congruence.
+      rewrite productNEqB_intro; try congruence.
+      rewrite orb_false_l in H1.
+      rewrite orb_false_l. auto.
+
+      destruct y; tinv H.
+      apply orb_true_iff in H1.
+      destruct H1 as [H1 | H1].
+        apply productEqB_inv in H1. inv H1.
+        erewrite FSim.(det_right) with (f1:=f0)(f2:=f2)(f:=f); eauto.
+        rewrite productEqB_refl. auto.
+
+        rewrite IHForall2; auto.
+        apply orb_true_r.
+Qed.
+
+Lemma system_simulation__getParentOfFdefFromSystem: forall S1 S2 f1 f2 m2
+  fid (Hsim: system_simulation S1 S2)
+  (Hfsim: FSim.(fsim) f1 f2)
+  (Hparent: getParentOfFdefFromSystem f2 S2 = Some m2)
+  (Hlkup: lookupFdefViaIDFromSystem S1 fid = ret f1),
+  exists m1, getParentOfFdefFromSystem f1 S1 = Some m1 /\
+             module_simulation m1 m2.
+Proof.
+  intros.
+  assert (J:=Hlkup).
+  apply lookupFdefViaIDFromSystem_ideq in J. subst.
+  induction Hsim; simpl in *; intros.
+    congruence.
+
+    match goal with
+    | H: match ?x with
+         | module_intro _ _ _ => 
+             match ?y with | module_intro _ _ _ => _ end
+         end |- _ => 
+        destruct x as [los1 nts1 Ps1]; destruct y as [los2 nts2 Ps2];
+        destruct H as [J1 [J2 J3]]; subst
+    end.
+    simpl in *.
+    assert (J:=Hfsim).
+    apply fdef_simulation__inv in J.
+    destruct_if.
+      destruct_match; simpl in e.       
+        exists (module_intro los2 nts2 Ps1).
+        split; simpl; auto.
+          match goal with
+          | |- (if ?e then _ else _ ) = _ => destruct e; auto
+          end.
+          simpl in e0. 
+          apply lookupFdefViaIDFromProducts__InProductsB in HeqR0.
+          congruence.
+
+          match goal with
+          | e: InProductsB (product_fdef ?f2) ?Ps2 = true,
+            HeqR0: None = lookupFdefViaIDFromProducts ?Ps1 (getFdefID ?f1),
+            J3: products_simulation ?Ps1 ?Ps2,
+            J: getFdefID ?f1 = getFdefID ?f2 |- _ =>
+            symmetry in HeqR0;
+            apply lookupFdefViaIDFromProducts__notin_getFdefsIDs in HeqR0;
+            assert (Hin:=e);  
+            apply InProductsB__in_getFdefsIDs in Hin;
+            apply products_simulation__eq_getFdefsIDs in J3;
+            simpl in Hin; rewrite J in HeqR0; congruence
+          end.
+
+      simpl in e.       
+      destruct_match.
+        apply lookupFdefViaIDFromProducts__InProductsB in HeqR0.
+        eapply products_fdef_simulation__InProductsB_forward in HeqR0; eauto.
+        congruence.
+
+        apply IHHsim in H0; auto.
+        destruct H0 as [m1 [J1 J2]].
+        exists m1.
+          split; auto. 
+          match goal with
+          | |- (if ?e then _ else _ ) = _ => destruct e; auto
+          end.
+          simpl in e0. 
+          assert (Hin:=e0).  
+          apply InProductsB__in_getFdefsIDs in Hin.
+          symmetry in HeqR0.
+          apply lookupFdefViaIDFromProducts__notin_getFdefsIDs in HeqR0.
+          simpl in Hin. rewrite J in HeqR0. congruence.
+Qed.
+
+Lemma genGlobalAndInitMem_spec_aux: forall td ps1 ps2 ,
+  products_simulation ps1 ps2 ->
+  forall gl fs M gl2 fs2 M2,
+  OpsemAux.genGlobalAndInitMem td ps2 gl fs M =
+    ret (gl2, fs2, M2) ->
+  exists gl1, exists fs1, exists M1,
+    OpsemAux.genGlobalAndInitMem td ps1 gl fs M =
+      ret (gl1, fs1, M1) /\ gl1 = gl2 /\ fs1 = fs2 /\ M1 = M2.
+Proof.
+  induction 1; intros.
+    fill_ctxhole. eauto 7.
+
+    destruct x; subst; simpl in *.
+      match goal with
+      | g:gvar |- _ => destruct g
+      end; inv_mbind; try destruct_let; eauto.
+        destruct f as [[]].
+        inv_mbind. eauto.
+
+      destruct f as [[]].
+      destruct y; simpl in *; tinv H.
+      destruct f0 as [[]].
+      inv_mbind. 
+      apply FSim.(eq_fheader) in H.
+      inv H. symmetry_ctx. fill_ctxhole. eauto.
+Qed.
+
+Lemma genGlobalAndInitMem_spec: forall td ps1 ps2 gl2 fs2 M2,
+  OpsemAux.genGlobalAndInitMem td ps2 nil nil Mem.empty =
+    ret (gl2, fs2, M2) ->
+  products_simulation ps1 ps2 ->
+  exists gl1, exists fs1, exists M1,
+    OpsemAux.genGlobalAndInitMem td ps1 nil nil Mem.empty =
+      ret (gl1, fs1, M1) /\ gl1 = gl2 /\ fs1 = fs2 /\ M1 = M2.
+Proof.
+  intros.
+  eapply genGlobalAndInitMem_spec_aux; eauto.
+Qed.
+
+Lemma lookupFdefViaPtr__simulation_None_l2r : forall Ps1 Ps2 fptr fs,
+  OpsemAux.lookupFdefViaPtr Ps2 fs fptr = None ->
+  products_simulation Ps1 Ps2 ->
+  OpsemAux.lookupFdefViaPtr Ps1 fs fptr = None.
+Proof.
+  intros.
+  unfold OpsemAux.lookupFdefViaPtr in *.
+  remember (OpsemAux.lookupFdefViaGVFromFunTable fs fptr) as R2.
+  destruct R2 as [fid|]; simpl in *; auto.
+  eapply products_simulation__fdef_None_r2l; eauto.
+Qed.
+
+Lemma lookupFdefViaPtr__simulation_None_r2l : forall Ps1 Ps2 fptr fs,
+  OpsemAux.lookupFdefViaPtr Ps1 fs fptr = None ->
+  products_simulation Ps1 Ps2 ->
+  OpsemAux.lookupFdefViaPtr Ps2 fs fptr = None.
+Proof.
+  intros.
+  unfold OpsemAux.lookupFdefViaPtr in *.
+  remember (OpsemAux.lookupFdefViaGVFromFunTable fs fptr) as R2.
+  destruct R2 as [fid|]; simpl in *; auto.
+  eapply products_simulation__fdef_None_l2r; eauto.
+Qed.
+
+Lemma products_simulation__fdec_None_r2l : forall fid Ps1 Ps2,
+  products_simulation Ps1 Ps2 ->
+  lookupFdecViaIDFromProducts Ps2 fid = None ->
+  lookupFdecViaIDFromProducts Ps1 fid = None.
+Proof.
+  intros.
+  erewrite products_simulation__fdec_eq; eauto. 
+Qed.
+
+Lemma products_simulation__fdec_None_l2r : forall fid Ps1 Ps2,
+  products_simulation Ps1 Ps2 ->
+  lookupFdecViaIDFromProducts Ps1 fid = None ->
+  lookupFdecViaIDFromProducts Ps2 fid = None.
+Proof.
+  intros.
+  erewrite <- products_simulation__fdec_eq; eauto. 
+Qed.
+
+Lemma lookupExFdecViaPtr__simulation_None_r2l : forall Ps1 Ps2 fptr fs,
+  OpsemAux.lookupExFdecViaPtr Ps2 fs fptr = None ->
+  products_simulation Ps1 Ps2 ->
+  OpsemAux.lookupExFdecViaPtr Ps1 fs fptr = None.
+Proof.
+  intros.
+  unfold OpsemAux.lookupExFdecViaPtr in *.
+  remember (OpsemAux.lookupFdefViaGVFromFunTable fs fptr) as R2.
+  destruct R2 as [fid|]; simpl in *; auto.
+  remember (lookupFdefViaIDFromProducts Ps2 fid) as R.
+  destruct R as [fid'|].
+    symmetry_ctx.
+    eapply products_simulation__fdef_simulation_r2l in HeqR; eauto.
+    destruct HeqR as [f1 [J1 J2]].
+    fill_ctxhole. auto.
+    erewrite products_simulation__fdef_None_r2l; eauto.
+
+  eapply products_simulation__fdec_None_r2l; eauto.
+Qed.
+
+Lemma lookupFdefViaPtr__simulation : forall Ps1 Ps2 fptr f1 f2 fs,
+  OpsemAux.lookupFdefViaPtr Ps2 fs fptr = Some f2 ->
+  products_simulation Ps1 Ps2 ->
+  OpsemAux.lookupFdefViaPtr Ps1 fs fptr = Some f1 ->
+  FSim.(fsim) f1 f2.
+Proof.
+  intros.
+  unfold OpsemAux.lookupFdefViaPtr in *.
+  remember (OpsemAux.lookupFdefViaGVFromFunTable fs fptr) as R2.
+  destruct R2 as [fid|]; inv H1. simpl in H.
+  eapply products_simulation__fdef_simulation in H0; eauto.
+Qed.
+
+Lemma lookupFdefViaPtr_inj__simulation : forall Ps1 Ps2 fptr1 fptr2 f1 f2 fs1
+  fs2 mi,
+  OpsemAux.ftable_simulation mi fs1 fs2 ->
+  OpsemAux.lookupFdefViaPtr Ps2 fs2 fptr2 = Some f2 ->
+  products_simulation Ps1 Ps2 ->
+  gv_inject mi fptr1 fptr2 ->
+  OpsemAux.lookupFdefViaPtr Ps1 fs1 fptr1 = Some f1 ->
+  FSim.(fsim) f1 f2.
+Proof.
+  intros.
+  unfold OpsemAux.lookupFdefViaPtr in *.
+  remember (OpsemAux.lookupFdefViaGVFromFunTable fs1 fptr1) as R1.
+  destruct R1 as [fid1|]; inv H3.
+  remember (OpsemAux.lookupFdefViaGVFromFunTable fs2 fptr2) as R2.
+  destruct R2 as [fid2|]; inv H0.
+  eapply products_simulation__fdef_simulation; eauto.
+  unfold OpsemAux.ftable_simulation in H.
+  erewrite H in HeqR1; eauto.
+  rewrite <- HeqR2 in HeqR1. inv HeqR1. auto.
+Qed.
+
+Lemma products_simulation__fdec_simulation : forall fid Ps1 Ps2
+  (Hsim: products_simulation Ps1 Ps2) f1 f2,
+  lookupFdecViaIDFromProducts Ps2 fid = Some f2 ->
+  lookupFdecViaIDFromProducts Ps1 fid = Some f1 ->
+  f1 = f2.
+Proof.
+  intros fid Ps1 Ps2 Hsim.
+  induction Hsim; simpl; intros.
+    inv H.
+
+    destruct x as [?|f|?];
+    destruct y as [?|f0|?]; inv H0; inv H1; eauto; try congruence.
+    destruct (getFdecID f0 == fid); subst.
+      inv H3.
+      destruct (getFdecID f == getFdecID f2).
+        inv H2. inv H. auto.
+
+        destruct f2 as [[]], f1 as [[]].
+        apply lookupFdecViaIDFromProducts_ideq in H2.
+        simpl in H2. subst.
+        destruct f.
+        inv H.
+        contradict n; auto.
+    destruct (getFdecID f == fid); subst; auto.
+      inv H2.
+      destruct f2 as [[]], f1 as [[]].
+      apply lookupFdecViaIDFromProducts_ideq in H3.
+      simpl in H3. subst.
+      destruct f0.
+      inv H.
+      contradict n; auto.
+Qed.
+
+Lemma lookupFdefViaPtr_inj__simulation_l2r : forall Ps1 Ps2 fptr1 fptr2 f1
+  fs1 fs2 mi f2,
+  products_simulation Ps1 Ps2 ->
+  OpsemAux.ftable_simulation mi fs1 fs2 ->
+  gv_inject mi fptr1 fptr2 ->
+  OpsemAux.lookupFdefViaPtr Ps1 fs1 fptr1 = Some f1 ->
+  OpsemAux.lookupExFdecViaPtr Ps2 fs2 fptr2 = Some f2 ->
+  False.
+Proof.
+  intros.
+  unfold OpsemAux.lookupFdefViaPtr in *.
+  remember (OpsemAux.lookupFdefViaGVFromFunTable fs1 fptr1) as R1.
+  destruct R1 as [fid1|]; inv H2.
+  unfold OpsemAux.lookupExFdecViaPtr in *.
+  remember (OpsemAux.lookupFdefViaGVFromFunTable fs2 fptr2) as R2.
+  destruct R2 as [fid2|]; inv H3.
+  remember (lookupFdefViaIDFromProducts Ps2 fid2) as R3.
+  destruct R3; inv H4.
+  eapply products_simulation__fdef_simulation_l2r in H5; eauto.
+  destruct H5 as [f2' [J1 J2]].
+  unfold OpsemAux.ftable_simulation in H0.
+  erewrite H0 in HeqR1; eauto.
+  rewrite <- HeqR1 in HeqR2. inv HeqR2.
+  rewrite J1 in HeqR3. inv HeqR3.
+Qed.
+
+Lemma lookupExFdecViaPtr_inj__simulation : forall Ps1 Ps2 fptr1 fptr2 f1
+  f2 fs1 fs2 mi,
+  products_simulation Ps1 Ps2 ->
+  OpsemAux.ftable_simulation mi fs1 fs2 ->
+  gv_inject mi fptr1 fptr2 ->
+  OpsemAux.lookupExFdecViaPtr Ps1 fs1 fptr1 = Some f1 ->
+  OpsemAux.lookupExFdecViaPtr Ps2 fs2 fptr2 = Some f2 ->
+  f1 = f2.
+Proof.
+  intros.
+  unfold OpsemAux.lookupExFdecViaPtr in *.
+  remember (OpsemAux.lookupFdefViaGVFromFunTable fs1 fptr1) as R1.
+  destruct R1 as [fid1|]; inv H2.
+  remember (lookupFdefViaIDFromProducts Ps1 fid1) as R3.
+  destruct R3; tinv H5.
+  remember (OpsemAux.lookupFdefViaGVFromFunTable fs2 fptr2) as R2.
+  destruct R2 as [fid2|]; inv H3.
+  remember (lookupFdefViaIDFromProducts Ps2 fid2) as R4.
+  destruct R4; tinv H4. symmetry_ctx.
+  unfold OpsemAux.ftable_simulation in H0.
+  erewrite H0 in HeqR1; eauto.
+  rewrite HeqR2 in HeqR1. inv HeqR1.
+  eapply products_simulation__fdec_simulation; eauto.
+Qed.
+
+Lemma lookupFdefViaPtr_inj__simulation_r2l : forall Ps1 Ps2 fptr1 fptr2 f1
+  fs1 fs2 mi f2,
+  products_simulation Ps1 Ps2 ->
+  OpsemAux.ftable_simulation mi fs1 fs2 ->
+  gv_inject mi fptr1 fptr2 ->
+  OpsemAux.lookupFdefViaPtr Ps2 fs2 fptr2 = Some f2 ->
+  OpsemAux.lookupExFdecViaPtr Ps1 fs1 fptr1 = Some f1 ->
+  False.
+Proof.
+  intros.
+  unfold OpsemAux.lookupFdefViaPtr in *.
+  remember (OpsemAux.lookupFdefViaGVFromFunTable fs2 fptr2) as R1.
+  destruct R1 as [fid2|]; inv H2.
+  unfold OpsemAux.lookupExFdecViaPtr in *.
+  remember (OpsemAux.lookupFdefViaGVFromFunTable fs1 fptr1) as R2.
+  destruct R2 as [fid1|]; inv H3.
+  remember (lookupFdefViaIDFromProducts Ps1 fid1) as R3.
+  destruct R3; inv H4.
+  eapply products_simulation__fdef_simulation_r2l in H5; eauto.
+  destruct H5 as [f2' [J1 J2]].
+  unfold OpsemAux.ftable_simulation in H0.
+  erewrite H0 in HeqR2; eauto.
+  rewrite <- HeqR2 in HeqR1. inv HeqR1.
+  rewrite J1 in HeqR3. inv HeqR3.
+Qed.
+
+Lemma lookupFdefViaPtr__simulation_l2r : forall Ps1 Ps2 fptr f1 fs,
+  products_simulation Ps1 Ps2 ->
+  OpsemAux.lookupFdefViaPtr Ps1 fs fptr = Some f1 ->
+  exists f2,
+    OpsemAux.lookupFdefViaPtr Ps2 fs fptr = Some f2 /\
+    FSim.(fsim) f1 f2.
+Proof.
+  unfold OpsemAux.lookupFdefViaPtr.
+  intros. 
+  destruct (OpsemAux.lookupFdefViaGVFromFunTable fs fptr); tinv H0.
+  simpl in H0.
+  eapply products_simulation__fdef_simulation_l2r in H0; eauto.
+Qed.
+
+Lemma lookupExFdecViaPtr__simulation_l2r : forall Ps1 Ps2 fptr f fs,
+  products_simulation Ps1 Ps2 ->
+  OpsemAux.lookupExFdecViaPtr Ps1 fs fptr = Some f ->
+  OpsemAux.lookupExFdecViaPtr Ps2 fs fptr = Some f.
+Proof.
+  unfold OpsemAux.lookupExFdecViaPtr.
+  intros. 
+  destruct (OpsemAux.lookupFdefViaGVFromFunTable fs fptr); tinv H0.
+  simpl in H0. simpl.
+  remember (lookupFdefViaIDFromProducts Ps1 i0) as R.
+  destruct R; tinv H0.
+  erewrite products_simulation__fdef_None_l2r; eauto.
+  erewrite products_simulation__fdec_l2r; eauto.
+Qed.
+
+Lemma lookupFdefViaPtr__simulation_r2l : forall Ps1 Ps2 fptr f2 fs,
+  products_simulation Ps1 Ps2 ->
+  OpsemAux.lookupFdefViaPtr Ps2 fs fptr = Some f2 ->
+  exists f1,
+    OpsemAux.lookupFdefViaPtr Ps1 fs fptr = Some f1 /\
+    FSim.(fsim) f1 f2.
+Proof.
+  unfold OpsemAux.lookupFdefViaPtr.
+  intros. 
+  destruct (OpsemAux.lookupFdefViaGVFromFunTable fs fptr); tinv H0.
+  simpl in H0.
+  eapply products_simulation__fdef_simulation_r2l in H0; eauto.
+Qed.
+
+Lemma lookupExFdecViaPtr__simulation_r2l : forall Ps1 Ps2 fptr f fs,
+  products_simulation Ps1 Ps2 ->
+  OpsemAux.lookupExFdecViaPtr Ps2 fs fptr = Some f ->
+  OpsemAux.lookupExFdecViaPtr Ps1 fs fptr = Some f.
+Proof.
+  unfold OpsemAux.lookupExFdecViaPtr.
+  intros. 
+  destruct (OpsemAux.lookupFdefViaGVFromFunTable fs fptr); tinv H0.
+  simpl in H0. simpl.
+  remember (lookupFdefViaIDFromProducts Ps2 i0) as R.
+  destruct R; tinv H0.
+  erewrite products_simulation__fdef_None_r2l; eauto.
+  erewrite products_simulation__fdec_r2l; eauto.
+Qed.
+
+End TopSim.
+
+End TopSim.
